Changed Axioms about external call

common/Events.v
@@ -616,6 +616,17 @@ Definition inject_separated (f f': meminj) (m1 m2: mem): Prop :=
   f b1 = None -> f' b1 = Some(b2, delta) ->
   ~Mem.valid_block m1 b1 /\ ~Mem.valid_block m2 b2.
 
+Definition external_block (b:block) : Prop :=
+  match b with
+    |Stack None _ _ => True
+    |_ => False
+  end.
+
+Definition inject_external (f: meminj) (m1 m2: mem): Prop :=
+  forall b,
+  ~ Mem.valid_block m1 b -> Mem.valid_block m2 b ->
+  external_block b /\ f b = Some (b,0).
+
 Record extcall_properties (sem: extcall_sem) (sg: signature) : Prop :=
   mk_extcall_properties {
 
