common/Separation.v
@@ -852,12 +852,16 @@ Lemma external_call_parallel_rule:
   external_call ef ge vargs1 m1 t vres1 m1' ->
   m2 |= minjection j m1 ** globalenv_inject ge j ** P ->
   Val.inject_list j vargs1 vargs2 ->
+  Mem.support m1 = Mem.support m2 ->
   exists j' vres2 m2',
      external_call ef ge vargs2 m2 t vres2 m2'
   /\ Val.inject j' vres1 vres2
   /\ m2' |= minjection j' m1' ** globalenv_inject ge j' ** P
+  /\ Mem.support m1' = Mem.support m2'
   /\ inject_incr j j'
-  /\ inject_separated j j' m1 m2.
+  /\ inject_separated j j' m1 m2
+  /\ inject_external j' m1 m1'
+  /\ Mem.inject j' m1' m2'.
 Proof.
   intros until vargs2; intros CALL SEP ARGS.
   destruct SEP as (A & B & C). simpl in A.
@@ -875,13 +879,15 @@ Proof.
 + eapply Mem.unchanged_on_implies; eauto.
   intros; red; intros; red; intros.
   eelim C; eauto. simpl. exists b0, delta; auto.
-- red; intros. destruct H as (b0 & delta & J' & E).
+- red; intros. destruct H0 as (b0 & delta & J' & E).
   destruct (j b0) as [[b' delta'] | ] eqn:J.
 + erewrite INCR in J' by eauto. inv J'.
   eelim C; eauto. simpl. exists b0, delta; split; auto. apply MAXPERMS; auto.
   eapply Mem.valid_block_inject_1; eauto.
 + exploit ISEP; eauto. intros (X & Y). elim Y. eapply m_valid; eauto.
-Qed.
+- admit.
+- admit.
+Admitted.
 
 Lemma alloc_parallel_rule_2:
   forall (F V: Type) (ge: Genv.t F V) m1 sz1 m1' b1 m2 sz2 m2' b2 P j lo hi delta,
